code/ecdsap256sha2/Hacl.Impl.P256.Signature.Common.fsti
@@ -18,7 +18,6 @@ open Hacl.Impl.P256
 
 open FStar.Mul
 
-
 (* This code is not side channel resistant *)
 (* inline_for_extraction noextract *)
 val eq_u64_nCT: a:uint64 -> b:uint64 -> (r:bool{r == (uint_v a = uint_v b)})
@@ -26,7 +25,6 @@ val eq_u64_nCT: a:uint64 -> b:uint64 -> (r:bool{r == (uint_v a = uint_v b)})
 (* This code is not side channel resistant *)
 (* inline_for_extraction noextract *)
 val eq_0_u64: a: uint64 -> r:bool{r == (uint_v a = 0)}
-
 
 val changeEndian: i:felem -> Stack unit 
   (requires fun h -> live h i)
@@ -39,15 +37,14 @@ val toUint64ChangeEndian: i:lbuffer uint8 (size 32) -> o:felem -> Stack unit
   (requires fun h -> live h i /\ live h o /\ disjoint i o)
   (ensures  fun h0 _ h1 ->
     modifies (loc o) h0 h1 /\
-    as_seq h1 o ==
-    Hacl.Spec.ECDSA.changeEndian (Lib.ByteSequence.uints_from_bytes_be (as_seq h0 i))
+    as_seq h1 o == Hacl.Spec.ECDSA.changeEndian (uints_from_bytes_be (as_seq h0 i))
   )
 
 val lemma_core_0: a:lbuffer uint64 (size 4) -> h:mem
   -> Lemma (nat_from_intseq_le (as_seq h a) == as_nat h a)
 
 val lemma_core_1: a:lbuffer uint64 (size 4) -> h:mem ->
-  Lemma (nat_from_bytes_le (Lib.ByteSequence.uints_to_bytes_le (as_seq h a)) == as_nat h a)
+  Lemma (nat_from_bytes_le (uints_to_bytes_le (as_seq h a)) == as_nat h a)
 
 val bufferToJac: p:lbuffer uint64 (size 8) -> result:point -> Stack unit
   (requires fun h -> live h p /\ live h result /\ disjoint p result)
